fpiwrgnprgnwpr

Games/gameLib_fixfix/Pairing.lean
@@ -10,41 +10,27 @@ import Games.gameLib_fixfix.Positional
 
 
 
+
 structure pairProp {win_sets : Finset (Finset α)} (win_set : win_sets) (p : α × α) : Prop where
   dif : p.1 ≠ p.2
   mem_fst : p.1 ∈ win_set.val
   mem_snd : p.2 ∈ win_set.val
 
 
-
-def pre_Pairing_condition [DecidableEq α] [Fintype α] (win_sets : Finset (Finset α)) : Prop :=
-   ∀ w : win_sets, ∃ p : α × α, pairProp w p
-
-
-noncomputable
-def pairing [DecidableEq α] [Fintype α] {win_sets : Finset (Finset α)} (h : pre_Pairing_condition win_sets) :=
-  @Classical.choose (win_sets → (α × α)) (fun f : win_sets → (α × α) => ∀ (x : { x // x ∈ win_sets }), pairProp x (f x)) (@Classical.axiomOfChoice _ _ pairProp h)
-
-
-lemma pairing_prop [DecidableEq α] [Fintype α] {win_sets : Finset (Finset α)} (h : pre_Pairing_condition win_sets) :
-  ∀ (x : { x // x ∈ win_sets }), pairProp x ((pairing h) x)  :=
-  @Classical.choose_spec (win_sets → (α × α)) (fun f : win_sets → (α × α) => ∀ (x : { x // x ∈ win_sets }), pairProp x (f x)) (@Classical.axiomOfChoice _ _ pairProp h)
-
 structure pairDif (a b : α × α) : Prop where
   strait_fst : a.1 ≠ b.1
-  strait_snd : a.1 ≠ b.1
+  strait_snd : a.2 ≠ b.2
   cross_fst : a.1 ≠ b.2
   cross_snd : a.2 ≠ b.1
 
-
-structure Pairing_condition [DecidableEq α] [Fintype α] (win_sets : Finset (Finset α)) where
-  has_pairing : pre_Pairing_condition win_sets
-  pairing_dif : ∀ w v : win_sets, w ≠ v → pairDif ((pairing has_pairing) w) ((pairing has_pairing) v)
+structure Pairing_condition [DecidableEq α] [Fintype α] (win_sets : Finset (Finset α)) (pairing : win_sets → (α × α)) where
+  has_pairing : ∀ w : win_sets, pairProp w (pairing w)
+  pairing_dif : ∀ w v : win_sets, w ≠ v → pairDif (pairing w) (pairing v)
 
 
 
 noncomputable
-def Pairing_StratCore [Inhabited α] [DecidableEq α] [Fintype α] {win_sets : Finset (Finset α)} (hg : Pairing_condition win_sets) :
+def Pairing_StratCore [Inhabited α] [DecidableEq α] [Fintype α] (win_sets : Finset (Finset α)) (pairing : win_sets → (α × α)) :
   (hist : List α) → (leg : Hist_legal (Positional_Game_World win_sets).init_game_state (Positional_Game_World win_sets).fst_legal (Positional_Game_World win_sets).snd_legal hist) → α :=
   fun hist leg =>
     let spam :=
@@ -55,16 +41,16 @@ def Pairing_StratCore [Inhabited α] [DecidableEq α] [Fintype α] {win_sets : F
               Classical.choose (((Positional_Game_World_playable win_sets) hist (leg)).2 (by rw [Turn_snd_iff_not_fst] ; exact T))
     match hist with
     | last :: _ =>
-        if hxf : ∃ w : win_sets, last = (pairing hg.has_pairing w).1
+        if hxf : ∃ w : win_sets, last = (pairing w).1
         then
-          let other := (pairing hg.has_pairing (Classical.choose hxf)).2
+          let other := (pairing (Classical.choose hxf)).2
           if other ∈ hist
           then spam
           else other
         else
-          if hxs : ∃ w : win_sets, last = (pairing hg.has_pairing w).2
+          if hxs : ∃ w : win_sets, last = (pairing w).2
           then
-            let other := (pairing hg.has_pairing (Classical.choose hxs)).1
+            let other := (pairing (Classical.choose hxs)).1
             if other ∈ hist
             then spam
             else other
@@ -76,53 +62,50 @@ def Pairing_StratCore [Inhabited α] [DecidableEq α] [Fintype α] {win_sets : F
 
 
 noncomputable
-def Pairing_fStrat [Inhabited α] [DecidableEq α] [Fintype α] {win_sets : Finset (Finset α)}  (hg : Pairing_condition win_sets) :
+def Pairing_fStrat [Inhabited α] [DecidableEq α] [Fintype α] {win_sets : Finset (Finset α)} (pairing : win_sets → (α × α)):
   fStrategy (Positional_Game_World win_sets).init_game_state (Positional_Game_World win_sets).fst_legal (Positional_Game_World win_sets).snd_legal :=
   fun hist T leg =>
-    ⟨ Pairing_StratCore hg hist leg,
+    ⟨ Pairing_StratCore win_sets pairing hist leg,
       (by
        dsimp [Positional_Game_World]
        split_ifs with N
        cases' hist with last L
        · dsimp [Pairing_StratCore]
          rw [dif_pos (by decide)]
-         exact
-           List.not_mem_nil
-             (Classical.choose
-               (Pairing_StratCore.proof_1 [] leg (of_decide_eq_true (Eq.refl true))))
+         apply List.not_mem_nil
        · dsimp [Pairing_StratCore]
-         by_cases hxf : ∃ w : win_sets, last = (pairing hg.has_pairing w).1
+         by_cases hxf : ∃ w : win_sets, last = (pairing w).1
          · rw [dif_pos hxf]
            split_ifs with M
-           · have := Classical.choose_spec (Pairing_StratCore.proof_1 (last :: L) leg (T))
+           · have := Classical.choose_spec (Pairing_StratCore.proof_1 win_sets (last :: L) leg (T))
              dsimp [Positional_Game_World] at this
              rw [if_pos N] at this
              exact this
-           · have := Classical.choose_spec (Pairing_StratCore.proof_1 (last :: L) leg (T))
+           · have := Classical.choose_spec (Pairing_StratCore.proof_1 win_sets (last :: L) leg (T))
              dsimp [Positional_Game_World] at this
              rw [if_pos N] at this
              exact this
            · exact M
          · rw [dif_neg hxf]
-           by_cases hxs : ∃ w : win_sets, last = (pairing hg.has_pairing w).2
+           by_cases hxs : ∃ w : win_sets, last = (pairing w).2
            · rw [dif_pos hxs]
              split_ifs with M
-             · have := Classical.choose_spec (Pairing_StratCore.proof_1 (last :: L) leg (T))
+             · have := Classical.choose_spec (Pairing_StratCore.proof_1 win_sets (last :: L) leg (T))
                dsimp [Positional_Game_World] at this
                rw [if_pos N] at this
                exact this
-             · have := Classical.choose_spec (Pairing_StratCore.proof_1 (last :: L) leg (T))
+             · have := Classical.choose_spec (Pairing_StratCore.proof_1 win_sets (last :: L) leg (T))
                dsimp [Positional_Game_World] at this
                rw [if_pos N] at this
                exact this
              · exact M
            · rw [dif_neg hxs]
              split_ifs with M
-             · have := Classical.choose_spec (Pairing_StratCore.proof_1 (last :: L) leg (T))
+             · have := Classical.choose_spec (Pairing_StratCore.proof_1 win_sets (last :: L) leg (T))
                dsimp [Positional_Game_World] at this
                rw [if_pos N] at this
                exact this
-             · have := Classical.choose_spec (Pairing_StratCore.proof_1 (last :: L) leg (T))
+             · have := Classical.choose_spec (Pairing_StratCore.proof_1 win_sets (last :: L) leg (T))
                dsimp [Positional_Game_World] at this
                rw [if_pos N] at this
                exact this
@@ -131,53 +114,50 @@ def Pairing_fStrat [Inhabited α] [DecidableEq α] [Fintype α] {win_sets : Fins
 
 
 noncomputable
-def Pairing_sStrat [Inhabited α] [DecidableEq α] [Fintype α] {win_sets : Finset (Finset α)}  (hg : Pairing_condition win_sets) :
+def Pairing_sStrat [Inhabited α] [DecidableEq α] [Fintype α] (win_sets : Finset (Finset α)) (pairing : win_sets → (α × α)) :
   sStrategy (Positional_Game_World win_sets).init_game_state (Positional_Game_World win_sets).fst_legal (Positional_Game_World win_sets).snd_legal :=
   fun hist T leg =>
-    ⟨ Pairing_StratCore hg hist leg,
+    ⟨ Pairing_StratCore win_sets pairing hist leg,
       (by
        dsimp [Positional_Game_World]
        split_ifs with N
        cases' hist with last L
        · dsimp [Pairing_StratCore]
          rw [dif_pos (by decide)]
-         exact
-           List.not_mem_nil
-             (Classical.choose
-               (Pairing_StratCore.proof_1 [] leg (of_decide_eq_true (Eq.refl true))))
+         apply List.not_mem_nil
        · dsimp [Pairing_StratCore]
-         by_cases hxf : ∃ w : win_sets, last = (pairing hg.has_pairing w).1
+         by_cases hxf : ∃ w : win_sets, last = (pairing w).1
          · rw [dif_pos hxf]
            split_ifs with M
-           · have := Classical.choose_spec (Pairing_StratCore.proof_2 (last :: L) leg (T))
+           · have := Classical.choose_spec (Pairing_StratCore.proof_2 win_sets (last :: L) leg (T))
              dsimp [Positional_Game_World] at this
              rw [if_pos N] at this
              exact this
-           · have := Classical.choose_spec (Pairing_StratCore.proof_2 (last :: L) leg (T))
+           · have := Classical.choose_spec (Pairing_StratCore.proof_2 win_sets (last :: L) leg (T))
              dsimp [Positional_Game_World] at this
              rw [if_pos N] at this
              exact this
            · exact M
          · rw [dif_neg hxf]
-           by_cases hxs : ∃ w : win_sets, last = (pairing hg.has_pairing w).2
+           by_cases hxs : ∃ w : win_sets, last = (pairing w).2
            · rw [dif_pos hxs]
              split_ifs with M
-             · have := Classical.choose_spec (Pairing_StratCore.proof_2 (last :: L) leg (T))
+             · have := Classical.choose_spec (Pairing_StratCore.proof_2 win_sets (last :: L) leg (T))
                dsimp [Positional_Game_World] at this
                rw [if_pos N] at this
                exact this
-             · have := Classical.choose_spec (Pairing_StratCore.proof_2 (last :: L) leg (T))
+             · have := Classical.choose_spec (Pairing_StratCore.proof_2 win_sets (last :: L) leg (T))
                dsimp [Positional_Game_World] at this
                rw [if_pos N] at this
                exact this
              · exact M
            · rw [dif_neg hxs]
              split_ifs with M
-             · have := Classical.choose_spec (Pairing_StratCore.proof_2 (last :: L) leg (T))
+             · have := Classical.choose_spec (Pairing_StratCore.proof_2 win_sets (last :: L) leg (T))
                dsimp [Positional_Game_World] at this
                rw [if_pos N] at this
                exact this
-             · have := Classical.choose_spec (Pairing_StratCore.proof_2 (last :: L) leg (T))
+             · have := Classical.choose_spec (Pairing_StratCore.proof_2 win_sets (last :: L) leg (T))
                dsimp [Positional_Game_World] at this
                rw [if_pos N] at this
                exact this
@@ -204,225 +184,11 @@ This is gonna ake ages
 
 
 
-theorem Pairing_Strategy [Inhabited α] [DecidableEq α] [Fintype α] {win_sets : Finset (Finset α)}  (hg : Pairing_condition win_sets) :
+theorem Pairing_Strategy [Inhabited α] [DecidableEq α] [Fintype α] {win_sets : Finset (Finset α)} {pairing : win_sets → (α × α)} (hg : Pairing_condition win_sets pairing) :
   (Positional_Game_World win_sets).is_draw_at_worst_snd :=
   by
-  use Pairing_sStrat hg
+  use Pairing_sStrat win_sets pairing
   intro f_strat
   sorry
 
 #check Game_wDraw.draw
-
-
-
-#exit
-
--- # Alternative
-
-structure pairDif (a b : α × α) : Prop where
-  strait_fst : a.1 ≠ b.1
-  strait_snd : a.1 ≠ b.1
-  cross_fst : a.1 ≠ b.2
-  cross_snd : a.2 ≠ b.1
-
-structure Pairing_condition [DecidableEq α] [Fintype α] {win_sets : Finset (Finset α)} (g : Positional_Game_World win_sets) where
-  playable : g.playable
-  pairing : List (α × α)
-  pairing_dif_inner : ∀ p ∈ pairing, p.1 ≠ p.2
-  pairing_dif_outer : List.Pairwise pairDif pairing
-  pairing_mem : ∀ w ∈ win_sets, ∃ n : Fin pairing.length, (pairing.get n).1 ∈ w ∧ (pairing.get n).2 ∈ w
-  -- should make the paring strat computable, if the element chosen in by playability are ... (via List.find?)
-  -- probably makes proofs of pairing_mem much more difficult ; I believe Hall is non-constructive in mathlib, so whats the point anyway
-
-
-
-
--- Initial stuff
-#exit
-
-structure Game_World.pairing_prop_pairdiff_fst
-  (g : Game_World (γ → Fin 3) γ)
-  (p : (s : (γ → Fin 3)) → (hw : g.fst_win_states s) → (γ × γ))
-  (w' v : (γ → Fin 3))
-  (hw' : fst_win_states g w')
-  (hv : fst_win_states g v)
-  : Prop where
-  d2 : (p w' hw).1 ≠ (p v hv).1
-  d3 : (p w' hw).2 ≠ (p v hv).2
-  d4 : (p w' hw).1 ≠ (p v hv).2
-  d5 : (p w' hw).2 ≠ (p v hv).1
-
-structure Game_World.pairing_prop_fst
-  (g : Game_World (γ → Fin 3) γ)
-  (p : (s : (γ → Fin 3)) → (hw : g.fst_win_states s) → (γ × γ))
-  (w' : (γ → Fin 3))
-  (hw' : fst_win_states g w')
-  : Prop where
-  d : (p w' hw').1 ≠ (p w' hw').2
-  ff : (w' (p w' hw').1 = 1)
-  sf : (w' (p w' hw').2 = 1)
-
-
-def Game_World.pairing_fst
-  (g : Game_World (γ → Fin 3) γ)
-  (p : (s : (γ → Fin 3)) → (hw : g.fst_win_states s) → (γ × γ))  : Prop :=
-    (∀ (w' : (γ → Fin 3)), (hw' : g.fst_win_states w') →
-      ( g.pairing_prop_fst p w' hw' ∧
-        (∀ (v : (γ → Fin 3)), (hv : g.fst_win_states v) → v ≠ w' →
-          g.pairing_prop_pairdiff_fst p w' v hw' hv)))
-
-
-def Game_World.has_pairing_fst
-  (g : Game_World (γ → Fin 3) γ) : Prop :=
-  ∃ p : (s : (γ → Fin 3)) → (hw : g.fst_win_states s) → (γ × γ),
-    g.pairing_fst p
-
-def Game_World.pairing_pairs
-  (g : Game_World (γ → Fin 3) γ)
-  (p : (s : (γ → Fin 3)) → (hw : g.fst_win_states s) → (γ × γ)) :
-  Set γ :=
-  {pts : γ | ∃ s : (γ → Fin 3), ∃ hw : g.fst_win_states s,  pts = (p s hw).1 ∨ pts = (p s hw).2}
-
-
-open Classical
-
-noncomputable
-def Game_World.snd_pairing_strat
-  [Inhabited γ]
-  (g : Game_World (γ → Fin 3) γ)
-  (p : (s : (γ → Fin 3)) → (hw : g.fst_win_states s) → (γ × γ))
-  : Strategy (γ → Fin 3) γ :=
-  fun ini hist =>
-    match hist with
-    | [] => default
-    | prev :: h => if h_mem : prev ∈ g.pairing_pairs p
-                   then (show γ from (
-                      by
-                      dsimp [Game_World.pairing_pairs] at h_mem
-                      choose s hw prop using h_mem
-                      -- cases' prop with
-                      -- · sorry -- expected checkColGt
-                      -- · sorry
-                      by_cases q :  prev = (p s hw).1 -- if prev is fst of pair
-                      · by_cases k : ∃ a : γ, a ∉ (prev :: h) -- if there are tiles left
-                        · by_cases K : (p s hw).2 ∉ (prev :: h) -- if the second of pair isn't taken
-                          · exact (p s hw).2 --then select second of pair
-                          · choose a _ using k -- else chose some available tile
-                            exact a
-                        · exact default -- should never occur
-                      · rw [or_iff_right q] at prop
-                        exact (p s hw).1 -- else choose first tile
-
-                   ))
-                   else (show γ from (
-                          by
-                          by_cases k : ∃ a : γ, a ∉ (prev :: h)
-                          · choose a _ using k
-                            exact a
-                          · exact default
-                   ))
-
-#print Game_World.snd_pairing_strat
-
-theorem Game.has_pairing_invariant_part1
-  [Inhabited γ]
-  (g : Game (γ → Fin 3) γ)
-  (hp : g.has_pairing_fst)
-  {T : ℕ} (ht : g.must_terminate_before T)
-  (hlf : g.fst_legal = fun hist act => act ∉ hist) -- add pos game transition too ?
-  (hls : g.snd_legal = fun hist act => act ∉ hist)
-  (p : (s : (γ → Fin 3)) → (hw : g.fst_win_states s) → (γ × γ))
-  (hp : g.pairing_fst p)
-  (hss : g.snd_strat = g.snd_pairing_strat p)
-  (special : ¬ (g.fst_win_states g.init_game_state))
-  :
-  ∀ turn : ℕ, (w : g.fst_win_states (g.state_on_turn turn)) →
-  (g.state_on_turn turn) (p (g.state_on_turn turn) w).1 = 1 →
-  (g.state_on_turn (turn + 1)) (p (g.state_on_turn (turn)) w).2 = 2 :=
-  by
-  intro t
-  induction' t with t ih
-  · dsimp [state_on_turn, history_on_turn, History_on_turn]
-    rw [if_pos (by decide)]
-    intro w fst_tile
-    exfalso
-    exact special w
-  · sorry
-
-
-
-#exit
-
-theorem Game.has_pairing_invariant
-  [Inhabited γ]
-  (g : Game (γ → Fin 3) γ)
-  (hp : g.has_pairing_fst)
-  {T : ℕ} (ht : g.must_terminate_before T)
-  (hlf : g.fst_legal = fun hist act => act ∉ hist) -- add pos game transition too ?
-  (hls : g.snd_legal = fun hist act => act ∉ hist)
-  (p : (s : (γ → Fin 3)) → (hw : g.fst_win_states s) → (γ × γ))
-  (hp : g.pairing_fst p)
-  (hss : g.snd_strat = g.snd_pairing_strat p)
-  (nontrivial : ¬ g.fst_win_states (g.fst_transition [] (g.fst_strat g.init_game_state []) )):
-  ∀ turn : ℕ, g.snd_win_states (g.state_on_turn turn) ∨ g.state_on_turn_neutral turn :=
-  by
-  intro t
-  apply @Nat.induct_2_step (fun t => Game_World.snd_win_states g.toGame_World (state_on_turn g t) ∨ state_on_turn_neutral g t)
-  · dsimp [state_on_turn, state_on_turn_neutral]
-    rw [if_neg (by decide)]
-    apply Classical.em
-  · dsimp [state_on_turn, state_on_turn_neutral]
-    rw [if_pos (by decide), if_pos (by decide), history_on_turn, History_on_turn]
-    right
-    exact nontrivial
-  · intro n c1 c2
-    rw [or_iff_not_imp_left]
-    intro c3
-    dsimp [state_on_turn_neutral]
-    split_ifs with tn
-    · intro con
-      specialize hp (state_on_turn g (n + 2)) con
-      obtain ⟨⟨h_d, h_ff, h_sf ⟩, h_diff⟩ := hp
-      -- unfold snd_strat to pairing strat to derive contra...
-    · exact c3
-
-#check Nat.induct_2_step
-
-#exit
-
-
-theorem Game_World.has_pairing_is_snd_draw
-  (g : Game_World (γ → Fin 3) γ)
-  (hp : g.has_pairing_fst)
-  {T : ℕ} (ht : g.must_terminate_before T)
-  (hlf : g.fst_legal = fun hist act => act ∉ hist) -- add pos game transition too ?
-  (hls : g.snd_legal = fun hist act => act ∉ hist) :
-  g.is_snd_win ∨ g.is_snd_draw :=
-  by
-  sorry
-
-
-
-#exit
-
--- Positional version:
-
-structure pairing_prop_aux
-  (win_sets : Finset (Finset α))
-  (p : (w : Finset α) → (hw : w ∈ win_sets) → (α × α))
-  (w' v : Finset α)
-  (hw : w' ∈ win_sets)
-  (hv : v ∈ win_sets)
-  : Prop where
-  d2 : (p w' hw).1 ≠ (p v hv).1
-  d3 : (p w' hw).2 ≠ (p v hv).2
-  d4 : (p w' hw).1 ≠ (p v hv).2
-  d5 : (p w' hw).2 ≠ (p v hv).1
-
-
-def Positional_Game_World.has_pairing (win_sets : Finset (Finset α)) :=
-  ∃ p : (w : Finset α) → (hw : w ∈ win_sets) → (α × α),
-    ∀ w' : Finset α, (hw : w' ∈ win_sets) →
-      ((p w' hw).1 ≠ (p w' hw).2) ∧
-      (∀ v : Finset α, (hv : v ∈ win_sets) → v ≠ w' →
-          pairing_prop_aux win_sets p w' v hw hv)
